LwRust.lean
@@ -1,9 +1,2 @@
 -- This module serves as the root of the `LwRust` library.
-import LwRust.Core.Syntax
-import LwRust.Core.ProgramSpace
 import LwRust.Paper
-import LwRust.Extensions.Tuples
-import LwRust.Extensions.ControlFlow
-import LwRust.Extensions.Functions
-import LwRust.Tests.Core
-import LwRust.Tests.Extensions
